treecp2
git-svn-id: svn://scm.gforge.inria.fr/svn/cfml@173 ba02c806-7d2b-4818-9a48-35b22e6bdc79

imper/TreeCopy.ml
@@ -1,9 +1,9 @@
 open MyLib
 
-type 'a tree = ('a * 'a tree * 'a tree) ref
+type 'a mtree = ('a * 'a mtree * 'a mtree) ref
 
-let copy_tree (copy_elem : 'a->'a) (t:'a tree) : 'a tree =
-  let rec copy (t:'a tree) : 'a tree =
+let copy_tree (copy_elem : 'a->'a) (t:'a mtree) : 'a mtree =
+  let rec copy (t:'a mtree) : 'a mtree =
      if t == null then null else
      let (x,t1,t2) = !t in
      ref (copy_elem x, copy t1, copy t2)
