imper/TreeCopy_proof.v
@@ -77,9 +77,11 @@ Inductive tree A :=
   | Leaf : tree A
   | Node : A -> tree A -> tree A -> tree A.
 
+Implicit Arguments Leaf [[A]].
+
 Fixpoint Tree A a (T:htype A a) (t:tree A) (l:loc) : hprop :=
   match t with
-  | Leaf => [l == null]
+  | Leaf => [l = null]
   | Node x t1 t2 => l ~> Ref3 T (Tree T) (Tree T) x t1 t2
   end.
 
@@ -93,7 +95,117 @@ Definition TreeSet A a (T:htype A a) (E:set A) (l:loc) :=
   Hexists (t:tree A), l ~> Tree T t \* [E = tree_set t].
   
 
-Lemma copy_tree_spec : forall a,
-  Spec ListRev_ml.rev (l:mlist a) |R>> forall A (T:A->a->hprop) (L:list A),
-     R (l ~> List T L) (~> List T (LibList.rev L)).
+Lemma focus_leaf : forall A a (T:A->a->hprop),
+  [] ==> null ~> Tree T Leaf.
+Proof. intros. simpl. hdata_simpl. hsimpl~. Qed.
+
+Lemma unfocus_leaf : forall (l:loc) A a (T:A->a->hprop),
+  l ~> Tree T Leaf ==> [l = null].
+Proof. intros. simpl. hdata_simpl. hsimpl~. Qed.
+
+Lemma unfocus_leaf' : forall A (t:tree A) a (T:A->a->hprop),
+  null ~> Tree T t ==> [t = Leaf].
 Proof.
+  intros. destruct t.
+  simpl. unfold hdata. xsimpl~.
+  skip. (* todo: focus_ref'  
+  unfold hdata, Tree. hchange (focus_ref_null). hextract. false. *)
+Qed.
+
+(* todo: qui l'a remis transparent?.  ==> fixer les preuves plus haut avec *)
+Opaque Ref.
+
+Lemma focus_node : forall (l:loc) a A (x:A) (t1 t2:tree A) (T:A->a->hprop),
+  l ~> Tree T (Node x t1 t2) ==>
+  Hexists (lx:a) (lt1:loc) (lt2:loc),
+  l ~> Ref Id (lx,lt1,lt2) \* (lx ~> T x) \* (lt1 ~> Tree T t1) \* (lt2 ~> Tree T t2).
+Proof.
+  intros. simpl. hdata_simpl. hchange (@focus_ref3 l).
+  hextract as x1 x2 x3. hsimpl.
+Qed.
+
+Lemma focus_node' : forall (l:loc) a A (t:tree A) (T:A->a->hprop),
+  [l <> null] \* (l ~> Tree T t) ==> 
+  Hexists (lx:a) (lt1:loc) (lt2:loc), Hexists (x:A) (t1:tree A) (t2:tree A),
+    l ~> Ref Id (lx,lt1,lt2) \* lx ~> T x \* lt1 ~> Tree T t1 \* lt2 ~> Tree T t2. 
+Proof.
+  intros. destruct t.
+  hextract. false. (* todo: simplifier dans focus_cons *)
+  hchange (@focus_node l). hextract as lx lt1 lt2 E. hsimpl~.  
+Qed.
+
+Lemma unfocus_node : forall (l:loc) a (lx:a) (lt1 lt2:loc) A (x:A) (t1 t2:tree A) (T:A->a->hprop),
+  l ~> Ref Id (lx,lt1,lt2) \* (lx ~> T x) \* (lt1 ~> Tree T t1) \* (lt2 ~> Tree T t2) ==>
+  l ~> Tree T (Node x t1 t2).
+Proof.
+  intros. simpl. hdata_simpl. hchange (@unfocus_ref3 l _ lx _ lt1 _ lt2). hsimpl.
+Qed.
+
+Opaque Tree.
+
+Inductive tree_sub {A} : binary (tree A) :=
+  | tree_sub_1 : forall x t1 t2,
+      tree_sub t1 (Node x t1 t2)
+  | tree_sub_2 : forall x t1 t2,
+      tree_sub t2 (Node x t1 t2).
+
+Lemma tree_sub_wf : forall A, wf (@tree_sub A).
+Proof.
+  intros A t. induction t; constructor; intros t' H; inversions~ H.
+Qed.
+
+Hint Resolve tree_sub_wf : wf.
+
+
+Ltac xbody_base_nointro tt ::=
+  xbody_core ltac:(fun _ => remove_head_unit tt).
+Tactic Notation "xfun_nointro" constr(s) :=
+  xfun_core s ltac:(fun _ => first [ xbody_base_nointro tt | xfun_namebody tt ] ).
+
+Tactic Notation "xapp" "as" simple_intropattern(x) :=
+  xlet as x; [ xapp | instantiate; xextract ].
+
+Lemma copy_tree_spec : forall a,
+  Spec copy_tree (copy_elem:val) (l:mtree a) |R>> 
+     forall A (T:A->a->hprop) (E:tree A),
+     (Spec copy_elem (x:a) |R>> forall X,
+        keep R (x ~> T X) (~> T X)) ->
+     keep R (l ~> Tree T E) (~> Tree T E).
+Proof.
+  xcf. introv Sce. 
+  xfun_nointro (fun f => Spec f (l:mtree a) |R>> forall E,
+           keep R (l ~> Tree T E) (~> Tree T E)).
+  skip IH: (Spec copy (l:mtree a) |R>> forall E,
+           keep R (l ~> Tree T E) (~> Tree T E)).
+  (* todo: induction *)
+    clear t E. intros t E.
+    xapp. intro_subst. xif.
+    xret. hchange (unfocus_leaf' E). hextract. subst. hsimpl~.
+     do 2 hchange focus_leaf. hsimpl.
+    xchange~ (@focus_node' t). xextract. intros lx lt1 lt2 x t1 t2.
+     xapp. intro_subst. xmatch.
+     xapp as lx'. 
+     xapp as lt1'.
+     xapp as lt2'.
+     xapp. intros r.
+      hchange_debug (@unfocus_node r _ lx' lt1' lt2').
+
+ hsimpl_setup tt.
+ hsimpl_step tt.
+ hsimpl_step tt.
+ hsimpl_step tt.
+ hsimpl_step tt.
+ hsimpl_step tt.
+
+ hsimpl_step tt.     
+  xapp. hsimpl.
+Qed.
+
+
+(* todo: spec with TreeSet *)
+(*(fun l' => l ~> Tree T E \* l' ~> Tree T E).*)
+
+
+
+
+
